src/QUIC.Impl.Header.fsti
@@ -15,14 +15,15 @@ module HS = FStar.HyperStack
 
 module Spec = QUIC.Spec.Header
 module Parse = QUIC.Spec.Header.Parse
-module AEAD = Spec.Agile.AEAD
+module SAEAD = Spec.Agile.AEAD
+module SCipher = Spec.Agile.Cipher
 
 module CTR = EverCrypt.CTR // because we do not want to friend the full state definition here
 
 unfold
 let header_encrypt_pre
   (a: ea)
-  (s: CTR.state (AEAD.cipher_alg_of_supported_alg a))
+  (s: CTR.state (SAEAD.cipher_alg_of_supported_alg a))
   (k: B.buffer Secret.uint8)
   (dst:B.buffer U8.t)
   (h: G.erased Spec.header)
@@ -33,7 +34,7 @@ let header_encrypt_pre
   (m: HS.mem)
 : GTot Type0
 =
-  let a' = AEAD.cipher_alg_of_supported_alg a in
+  let a' = SAEAD.cipher_alg_of_supported_alg a in
   let fmt = Parse.format_header h in
   let header_len = Seq.length fmt in
 
@@ -44,7 +45,7 @@ let header_encrypt_pre
   ] /\
 
   CTR.invariant m s /\
-  B.live m k /\ B.length k == Spec.Agile.Cipher.key_length a' /\
+  B.live m k /\ B.length k == SCipher.key_length a' /\
   B.live m dst /\
 
   is_short == Spec.MShort? h /\
@@ -64,7 +65,7 @@ let header_encrypt_pre
 unfold
 let header_encrypt_post
   (a: ea)
-  (s: CTR.state (AEAD.cipher_alg_of_supported_alg a))
+  (s: CTR.state (SAEAD.cipher_alg_of_supported_alg a))
   (k: B.buffer Secret.uint8)
   (dst:B.buffer U8.t)
   (h: G.erased Spec.header)
@@ -78,6 +79,116 @@ let header_encrypt_post
 = 
   header_encrypt_pre a s k dst h is_short is_retry public_len pn_len m /\
   begin
+    let a' = SAEAD.cipher_alg_of_supported_alg a in
+    let fmt = Parse.format_header h in
+    let header_len = Seq.length fmt in
+    let cipher = Seq.slice (B.as_seq m dst) header_len (B.length dst) in
+    B.modifies (B.loc_buffer dst `B.loc_union` CTR.footprint m s) m m' /\
+    B.as_seq m' dst `Seq.equal`
+      Spec.header_encrypt a (B.as_seq m k) h cipher /\
+    CTR.invariant m' s /\
+    CTR.footprint m s == CTR.footprint m' s
+  end
+
+val header_encrypt: a: ea ->
+  (s: CTR.state (SAEAD.cipher_alg_of_supported_alg a)) ->
+  (k: B.buffer Secret.uint8) ->
+  dst:B.buffer U8.t ->
+  h: G.erased Spec.header ->
+  is_short: bool ->
+  is_retry: bool ->
+  public_len: U32.t ->
+  pn_len: PN.packet_number_length_t ->
+  HST.Stack unit
+    (requires (fun h0 ->
+      header_encrypt_pre a s k dst h is_short is_retry public_len pn_len h0
+    ))
+    (ensures fun h0 _ h1 ->
+      header_encrypt_post a s k dst h is_short is_retry public_len pn_len h0 h1
+    )
+
+noeq
+type h_result =
+| H_Failure
+| H_Success:
+    (h: header) ->
+    (pn: PN.packet_number_t) ->
+    (cipher_length: Secret.uint32) ->
+    h_result
+
+unfold
+let header_decrypt_pre
+  (a: ea)
+  (s: CTR.state (SAEAD.cipher_alg_of_supported_alg a))
+  (k: B.buffer Secret.uint8)
+  (cid_len: short_dcid_len_t)
+  (last: PN.last_packet_number_t)
+  (dst:B.buffer U8.t)
+  (dst_len: U32.t)
+  (m: HS.mem)
+: GTot Type0
+=
+  let a' = SAEAD.cipher_alg_of_supported_alg a in
+  B.all_disjoint [
+    CTR.footprint m s;
+    B.loc_buffer k;
+    B.loc_buffer dst;
+  ] /\
+  CTR.invariant m s /\
+  B.live m k /\ B.length k == SCipher.key_length a' /\
+  B.live m dst /\ B.length dst == U32.v dst_len
+
+unfold
+let header_decrypt_post
+  (a: ea)
+  (s: CTR.state (SAEAD.cipher_alg_of_supported_alg a))
+  (k: B.buffer Secret.uint8)
+  (cid_len: short_dcid_len_t)
+  (last: PN.last_packet_number_t)
+  (dst:B.buffer U8.t)
+  (dst_len: U32.t)
+  (m: HS.mem)
+  (res: h_result)
+  (m' : HS.mem)
+: GTot Type0
+= 
+  header_decrypt_pre a s k cid_len last dst dst_len m /\
+  CTR.footprint m' s == CTR.footprint m s /\
+  CTR.invariant m' s /\
+  begin match res, Spec.header_decrypt a (B.as_seq m k) (U32.v cid_len) (Secret.v last) (B.as_seq m dst) with
+  | H_Failure, Spec.H_Failure ->
+    B.modifies B.loc_none m m'
+  | H_Success h pn cipher_len, Spec.H_Success gh gcipher grem ->
+    header_live h m' /\
+    gh == g_header h m' pn /\
+    Secret.v (header_len h) + Secret.v cipher_len <= B.length dst /\
+    B.loc_buffer (B.gsub dst 0ul (public_header_len h)) `B.loc_includes` header_footprint h /\
+    B.modifies (B.loc_buffer (B.gsub dst 0ul (Secret.reveal (header_len h))) `B.loc_union` CTR.footprint m s) m m' /\
+    Seq.length gcipher == Secret.v cipher_len /\
+    B.as_seq m' dst `Seq.equal` (Parse.format_header gh `Seq.append` gcipher `Seq.append` grem)
+  | _ -> False
+  end
+
+val header_decrypt
+  (a: ea)
+  (s: CTR.state (SAEAD.cipher_alg_of_supported_alg a))
+  (k: B.buffer Secret.uint8)
+  (cid_len: short_dcid_len_t)
+  (last: PN.last_packet_number_t)
+  (dst:B.buffer U8.t)
+  (dst_len: U32.t)
+: HST.Stack h_result
+  (requires (fun m ->
+    header_decrypt_pre a s k cid_len last dst dst_len m
+  ))
+  (ensures (fun m res m' ->
+    header_decrypt_post a s k cid_len last dst dst_len m res m'
+  ))
+
+
+(*
+
+
     let a' = AEAD.cipher_alg_of_supported_alg a in
     let fmt = Parse.format_header h in
     let header_len = Seq.length fmt in
@@ -105,6 +216,7 @@ val header_encrypt: a: ea ->
     (ensures fun h0 _ h1 ->
       header_encrypt_post a s k dst h is_short is_retry public_len pn_len h0 h1
     )
+
 
 (*
       let fmt = Parse.format_header h in
